compiler/backend/presLangScript.sml
@@ -660,6 +660,7 @@ val stack_prog_to_display_def = Define`
          asm_reg_imm_to_display to; stack_prog_to_display x]
     | JumpLower n1 n2 n3 => item_with_nums «JumpLower» [n1; n2; n3]
     | Alloc n => item_with_num «Alloc» n
+    | StoreConsts => empty_item «StoreConsts»
     | Raise n => item_with_num «Raise» n
     | Return n1 n2 => item_with_nums «Return» [n1; n2]
     | FFI nm cp cl ap al ra => Item NONE «FFI»
@@ -775,6 +776,8 @@ val word_prog_to_display_def = tDefine "word_prog_to_display" `
     [word_prog_to_display p1; word_prog_to_display p2]) /\
   (word_prog_to_display (Alloc n ns) = Item NONE (strlit "Alloc")
     [num_to_display n; num_set_to_display ns]) /\
+  (word_prog_to_display (StoreConsts a b c d ws) = Item NONE (strlit "StoreConsts")
+    [num_to_display a; num_to_display b; num_to_display c; num_to_display d] (* TODO: include ws *)) /\
   (word_prog_to_display (Raise n) = item_with_num (strlit "Raise") n) /\
   (word_prog_to_display (Return n1 n2) = item_with_nums (strlit "Return") [n1; n2]) /\
   (word_prog_to_display Tick = empty_item (strlit "Tick")) /\
